feat: fill out the basic top level definitions

Filrb/Basic.lean
@@ -1,4 +1,5 @@
-import Filrb.Internal
+import Filrb.Internal.Invariants
+import Filrb.Internal.Mem
 
 namespace Filrb
 
@@ -12,25 +13,46 @@ namespace Set
 
 variable [Preorder α] [Ord α] [LawfulOrd α]
 
-def empty : Set α := sorry
+def empty : Set α :=
+  {
+    raw := .nil
+    bst := Internal.Raw.bst_nil
+    color := Internal.Raw.childInv_nil
+    height := Internal.Raw.heightInv_nil
+  }
 
 instance : EmptyCollection (Set α) where
-  emptyCollection := sorry
+  emptyCollection := empty
 
-def isEmpty (s : Set α) : Bool := sorry
+def isEmpty (s : Set α) : Bool := s.raw.isEmpty
 
-def insert (set : Set α) (x : α) : Set α := sorry
+def insert (set : Set α) (x : α) : Set α :=
+  let ⟨raw, bst, color, height⟩ := set
+  {
+    raw := raw.insert x
+    bst := Internal.Raw.bst_insert_of_bst x raw bst
+    color := Internal.Raw.childInv_insert_of_bst x raw color
+    height := Internal.Raw.heightInv_insert_of_bst x raw height
+  }
 
-def contains (set : Set α) (x : α) : Bool := sorry
+def contains (set : Set α) (x : α) : Bool := set.raw.contains x
 
 instance : Membership α (Set α) where
-  mem := sorry
+  mem set x := x ∈ set.raw
 
-instance {x : α} {set : Set α} : Decidable (x ∈ set) := sorry
+instance {x : α} {set : Set α} : Decidable (x ∈ set) :=
+  decidable_of_iff (set.contains x) (Internal.Raw.contains_eq_true_iff_mem_of_bst set.bst)
 
-def erase (set : Set α) (x : α) : Set α := sorry
+def erase (set : Set α) (x : α) : Set α :=
+  let ⟨raw, bst, color, height⟩ := set
+  {
+    raw := raw.erase x
+    bst := Internal.Raw.bst_erase_of_bst x raw bst
+    color := Internal.Raw.childInv_erase_of_bst x raw color
+    height := Internal.Raw.heightInv_erase_of_bst x raw height
+  }
 
-def size (set : Set α) : Nat := sorry
+def size (set : Set α) : Nat := set.raw.size
 
 end Set
 
